Finish AST

ExtParser/AST.lean
@@ -25,11 +25,11 @@ namespace AST
     | ε : IsValid (.ε s e)
     | any : IsValid (.any s e x)
     | terminal : IsValid (.terminal s e a x)
-    | nonTerminal : IsValid T → ¬SkipPreAST' T → IsValid (.nonTerminal s e A T)
+    | nonTerminal : IsValid sub_T → ¬SkipPreAST' sub_T → IsValid (.nonTerminal s e A sub_T)
     | seq : IsValid T1 → IsValid T2 → ¬SkipPreAST' T1 → IsValid (.seq s e T1 T2)
     | prior : IsValid T1 → IsValid T2 → ¬SkipPreAST' T1 → IsValid (.prior s e T1 T2)
     | star : IsValid T0 → IsValid TS → ¬SkipPreAST' T0 → (SkipPreAST' TS ∨ StarPreAST' TS) → IsValid (.star s e T0 TS)
-    | notP : IsValid T → ¬SkipPreAST' T → IsValid (.notP s e T)
+    | notP : IsValid sub_T → ¬SkipPreAST' sub_T → IsValid (.notP s e sub_T)
 
   def PreAST'.size (T : PreAST' n b) : Nat :=
     match T with
@@ -43,10 +43,36 @@ namespace AST
     | .star _ _ T0 TS => T0.size + TS.size + 1
     | .notP _ _ T => T.size + 1
   
+  def PreAST'.start (T : PreAST' n b) : Fin b :=
+    match T with
+    | .skip s _ _             => s
+    | .ε s _                  => s
+    | .any s _ _              => s
+    | .terminal s _ _ _       => s
+    | .nonTerminal s _ _ _    => s
+    | .seq s _ _ _            => s
+    | .prior s _ _ _          => s
+    | .star s _ _ _           => s
+    | .notP s _ _             => s
+
+  def PreAST'.end (T : PreAST' n b) : Fin b :=
+    match T with
+    | .skip _ e _             => e
+    | .ε _ e                  => e
+    | .any _ e _              => e
+    | .terminal _ e _ _       => e
+    | .nonTerminal _ e _ _    => e
+    | .seq _ e _ _            => e
+    | .prior _ e _ _          => e
+    | .star _ e _ _           => e
+    | .notP _ e _             => e
 
   structure PreAST (n : Nat) (b : Nat) where
     T : PreAST' n b
     valid_T : PreAST'.IsValid T
+  
+  def PreAST.start (T : PreAST n b) : Fin b := T.T.start
+  def PreAST.end (T : PreAST n b) : Fin b := T.T.end
 
   mutual
 
@@ -251,5 +277,203 @@ namespace AST
           | .failure h => .success (.notP (h := g) h)
           | .undefined hs hf => .undefined (by intro h; cases h; contradiction) (by intro h; cases h; contradiction)
 
+  theorem PreAST.star_cannot_fail : ∀ {T : PreAST n b}, StarPreAST' T.T → ¬FailureAST T := by
+    intro T h_star h_fail;
+    match T with
+    | .mk T valid_T => simp_all; cases h_star; cases h_fail
+  
+  def PreAST.IsMeaningful (T : PreAST n b) : Prop := SuccessAST T ∨ FailureAST T
 
+  inductive PreAST.IsWellformed : PreAST n b → Prop where
+    | ε :           IsMeaningful (mk (.ε s e) h) 
+                    → IsWellformed (mk (.ε s e) h)
+    | any :         IsMeaningful (mk (.any s e x) h) 
+                    → IsWellformed (mk (.any s e x) h)
+    | terminal :    IsMeaningful (mk (.terminal s e a x) h) 
+                    → IsWellformed (mk (.terminal s e a x) h)
+    | nonTerminal : ∀ {sub_T : PreAST n b} {h : PreAST'.IsValid (PreAST'.nonTerminal s e A sub_T.T)},
+                    s = sub_T.start → e = sub_T.end 
+                    → IsWellformed sub_T 
+                    → IsWellformed (mk (.nonTerminal s e A sub_T.T) h)
+    | seq_F :       ∀ {T1 T2 : PreAST n b} {h : PreAST'.IsValid (PreAST'.seq s e T1.T T2.T)},
+                    s = T1.start → T1.end = T2.start → e = T2.end → T2.start = T2.end
+                    → IsWellformed T1 → FailureAST T1 → SkipPreAST' T2.T
+                    → IsWellformed (mk (.seq s e T1.T T2.T) h)
+    | seq_S :       ∀ {T1 T2 : PreAST n b} {h : PreAST'.IsValid (PreAST'.seq s e T1.T T2.T)},
+                    s = T1.start → T1.end = T2.start → e = T2.end 
+                    → IsWellformed T1 → SuccessAST T1 → IsWellformed T2
+                    → IsWellformed (mk (.seq s e T1.T T2.T) h)
+    | prior_S :     ∀ {T1 T2 : PreAST n b} {h : PreAST'.IsValid (PreAST'.prior s e T1.T T2.T)},
+                    s = T1.start → s = T2.start → s = T2.end → e = T1.end 
+                    → IsWellformed T1 → SuccessAST T1 → SkipPreAST' T2.T
+                    → IsWellformed (mk (.prior s e T1.T T2.T) h)
+    | prior_F :     ∀ {T1 T2 : PreAST n b} {h : PreAST'.IsValid (PreAST'.prior s e T1.T T2.T)},
+                    s = T1.start → s = T2.start → e = T2.end 
+                    → IsWellformed T1 → FailureAST T1 → IsWellformed T2
+                    → IsWellformed (mk (.prior s e T1.T T2.T) h)
+    | star_S :      ∀ {T0 TS : PreAST n b} {h : PreAST'.IsValid (PreAST'.star s e T0.T TS.T)},
+                    s = T0.start → T0.end = TS.start → e = TS.end
+                    → IsWellformed T0 → SuccessAST T0 → IsWellformed TS
+                    → IsWellformed (mk (.star s e T0.T TS.T) h)
+    | star_F :      ∀ {T0 TS : PreAST n b} {h : PreAST'.IsValid (PreAST'.star s e T0.T TS.T)},
+                    s = T0.start → T0.end = TS.start → TS.start = TS.end → s = e
+                    → IsWellformed T0 → FailureAST T0 → SkipPreAST' TS.T  
+                    → IsWellformed (mk (.star s e T0.T TS.T) h)
+    | notP :        ∀ {sub_T : PreAST n b} {h : PreAST'.IsValid (PreAST'.notP s e sub_T.T)},
+                    s = e → s = sub_T.start
+                    → IsWellformed sub_T 
+                    → IsWellformed (mk (.notP s e sub_T.T) h)
+
+  theorem PreAST.skip_is_not_wellformed : ∀ {T : PreAST n b}, SkipPreAST' T.T → ¬IsWellformed T := by
+    intro T h_skip hwf;
+    cases T; simp_all; cases h_skip; cases hwf;
+
+  theorem PreAST.wellformed_implies_meaningful : ∀ {T : PreAST n b}, IsWellformed T → IsMeaningful T := by
+    intro T hwf;
+    match hwf with
+    | .ε _ => assumption
+    | .any _ => assumption
+    | .terminal _ => assumption
+    | .nonTerminal (h := h_valid) _ _ hwfT =>
+      {
+        cases h_valid; cases wellformed_implies_meaningful hwfT;
+        apply Or.inl; constructor <;> assumption;
+        apply Or.inr; constructor <;> assumption;
+      }
+    | .seq_F (h := h_valid) _ _ _ _ _ hf1 hskip2 =>
+      {
+        cases h_valid; apply Or.inr;
+        apply FailureAST.seq_F <;> assumption;
+      }
+    | .seq_S (h := h_valid) _ _ _ _ hs1 hwf2 =>
+      {
+        cases h_valid; cases wellformed_implies_meaningful hwf2;
+        apply Or.inl; constructor <;> assumption;
+        apply Or.inr; apply FailureAST.seq_SF <;> assumption;
+      }
+    | .prior_S (h := h_valid) _ _ _ _ _ hs1 hskip2 =>
+      {
+        cases h_valid; apply Or.inl;
+        apply SuccessAST.prior_S <;> assumption;
+      }
+    | .prior_F (h := h_valid) _ _ _ _ hf1 hwf2 =>
+      {
+        cases h_valid; cases wellformed_implies_meaningful hwf2;
+        apply Or.inl; apply SuccessAST.prior_FS <;> assumption;
+        apply Or.inr; constructor <;> assumption;
+      }
+    | .star_S (TS := TS) (h := h_valid) _ _ _ _ hs0 hwfS =>
+      {
+        match h_valid with
+        | PreAST'.IsValid.star _ _ _ svs => 
+          match svs with
+          | Or.inl hskip =>
+            {
+              apply absurd hwfS;
+              apply skip_is_not_wellformed; assumption;
+            }
+          | Or.inr hstar =>
+            {
+              apply Or.inl; apply SuccessAST.star_SS;
+              assumption; apply Or.inr; assumption; assumption;
+              match wellformed_implies_meaningful hwfS with
+              | Or.inl _ => assumption
+              | Or.inr hf => cases TS; cases hstar; cases hf;
+            }
+        
+      }
+    | .star_F (h := h_valid) _ _ _ _ _ hf0 hskipS =>
+      {
+        cases h_valid; apply Or.inl;
+        apply SuccessAST.star_F <;> assumption;
+      }
+    | .notP (h := h_valid) _ _ hwfT =>
+      {
+        cases h_valid; cases wellformed_implies_meaningful hwfT;
+        apply Or.inr; constructor <;> assumption;
+        apply Or.inl; constructor <;> assumption;
+      }
+  
+  theorem PreAST.start_le_end : ∀ {T : PreAST n b}, IsWellformed T → T.start ≤ T.end := by
+    intro T hwf;
+    match hwf with
+    | .ε hm =>
+      {
+        cases T; simp [PreAST.start, PreAST.end, PreAST'.start, PreAST'.end];
+        match hm with
+        | Or.inl hs => cases hs; apply Nat.le_of_eq; apply Fin.val_eq_of_eq; assumption;
+      }
+    | .any hm =>
+      {
+        cases T; simp [PreAST.start, PreAST.end, PreAST'.start, PreAST'.end];
+        match hm with
+        | Or.inl hs => cases hs; apply Nat.le_of_lt; apply Fin.lt_from_inbound_succ; assumption;
+        | Or.inr hf => cases hf; apply Nat.le_of_eq; apply Fin.val_eq_of_eq; assumption;
+      }
+    | .terminal hm =>
+      {
+        cases T; simp [PreAST.start, PreAST.end, PreAST'.start, PreAST'.end];
+        match hm with
+        | Or.inl hs => cases hs; apply Nat.le_of_lt; apply Fin.lt_from_inbound_succ; assumption;
+        | Or.inr hf => cases hf; apply Nat.le_of_lt; apply Fin.lt_from_inbound_succ; assumption; apply Nat.le_of_eq; apply Fin.val_eq_of_eq; assumption;
+      }
+    | .nonTerminal (h := h_valid) hssT heeT hwfT =>
+      {
+        cases T; simp [PreAST.start, PreAST.end, PreAST'.start, PreAST'.end];
+        rw [hssT, heeT];
+        apply start_le_end;
+        assumption;
+      }
+    | .seq_F (h := h_valid) hss1 he1s2 hee2 hs2e2 hwf1 _ hskip2 =>
+      {
+        cases T; simp [PreAST.start, PreAST.end, PreAST'.start, PreAST'.end];
+        rw [hss1, hee2, ←hs2e2, ←he1s2]
+        apply start_le_end hwf1;
+      }
+    | .seq_S (h := h_valid) hss1 he1s2 hee2 hwf1 _ hwf2 =>
+      {
+        cases T; simp [PreAST.start, PreAST.end, PreAST'.start, PreAST'.end];
+        rw [hss1, hee2];
+        apply Nat.le_trans;
+        apply start_le_end hwf1;
+        rw [he1s2];
+        apply start_le_end hwf2;
+      }
+    | .prior_S (h := h_valid) hss1 _ _ hee1 hwf1 _ hskip2 =>
+      {
+        cases T; simp [PreAST.start, PreAST.end, PreAST'.start, PreAST'.end];
+        rw [hss1, hee1];
+        apply start_le_end hwf1;
+      }
+    | .prior_F (h := h_valid) _ hss2 hee2 _ _ hwf2 =>
+      {
+        cases T; simp [PreAST.start, PreAST.end, PreAST'.start, PreAST'.end];
+        rw [hss2, hee2];
+        apply start_le_end hwf2;
+      }
+    | .star_S (TS := TS) (h := h_valid) hss0 he0sS heeS hwf0 _ hwfS =>
+      {
+        cases T; simp [PreAST.start, PreAST.end, PreAST'.start, PreAST'.end];
+        rw [hss0, heeS];
+        apply Nat.le_trans;
+        apply start_le_end hwf0;
+        rw [he0sS];
+        apply start_le_end hwfS;
+      }
+    | .star_F (h := h_valid) _ _ _ hse _ _ hskipS =>
+      {
+        cases T; simp [PreAST.start, PreAST.end, PreAST'.start, PreAST'.end];
+        rw [hse];
+        apply Nat.le_refl;
+      }
+    | .notP (h := h_valid) hse _ hwfT =>
+      {
+        cases T; simp [PreAST.start, PreAST.end, PreAST'.start, PreAST'.end];
+        rw [hse];
+        apply Nat.le_refl;
+      }
+
+  structure AST (n : Nat) (b : Nat) where
+    T : PreAST n b
+    wf_T : PreAST.IsWellformed T
 end AST
